Pushed another bug to the reifier

examples/PolyApply/Test.v
@@ -58,148 +58,29 @@ Section Test.
   Proof.
     reflexivity.
   Qed.
- 
+
+  Definition reify_poly := reify_scheme@{Set} (expr typ func).
   Ltac reify_poly e :=
     let k e :=
         pose e in
-    reify_expr reify_eq k
+    reify_expr reify_poly k
                [[ True ]]
                [[ e ]].
 
   Goal True.
-    (* GREGORY, This breaks *)
-    reify_poly (forall P : nat, P = P).
+    (* This reifies *)
+    reify_poly (forall x : nat, x = x).
+    apply I.
+  Qed.
+    
 
   Definition lem_landexistsDL : 
     polymorphic typ 1
                 (Lemma.lemma typ (expr typ func) 
                              (rw_concl typ func (expr typ func))).   
   Proof.
+    (* But this does not *)
     Eval unfold Lemma.add_var, Lemma.add_prem , Lemma.vars , Lemma.concl , Lemma.premises in
         <:: @Id ::>.
   Qed.
     
-  
-
-Definition func_map :
-  OneOfType.pmap :=
-  list_to_pmap
-    (pcons (listOp_func typ)
-           (pcons (list_func typ)
-                  (pcons SymEnv.func
-                         (pcons natFunc
-                                pnil)))).
-
-Definition func := OneOf func_map.
-
-Global Instance TableView_func : PartialView func SymEnv.func :=
-  PartialViewPMap 3 func_map eq_refl.
-Global Instance NatView_func : PartialView func natFunc :=
-  PartialViewPMap 4 func_map eq_refl.
-Global Instance ListView_func : PartialView func (list_func typ) :=
-  PartialViewPMap 2 func_map eq_refl.
-Global Instance ListOpView_func : PartialView func (listOp_func typ) :=
-  PartialViewPMap 1 func_map eq_refl.
-
-Class Environment := { simple_env :> @SymEnv.functions typ _}.
-
-Existing Instance RelDec_from_RType.
-
-Section SimpleFunc.
-
-  Context {fs : Environment}.
-
-  Global Instance RSym_func : RSym func.
-  Proof.
-    apply RSymOneOf.
-    repeat first [eapply RSym_All_Branch_None |
-                  eapply RSym_All_Branch_Some |
-                  eapply RSym_All_Empty].
-
-    apply RSym_ListOpFunc.
-    apply RSym_ListFunc.
-    apply RSym_NatFunc.
-    apply RSym_func; apply fs.
-  Defined.
-
-  Global Instance RSymOk_func : RSymOk RSym_func.
-  apply RSymOk_OneOf.
-
-  repeat first [eapply RSymOk_All_Branch_None |
-                eapply RSymOk_All_Branch_Some; [apply _ | |] |
-                eapply RSymOk_All_Empty].
-  Defined.
-
-  Global Instance Expr_expr : ExprI.Expr _ (expr typ func) := @Expr_expr typ func _ _ _.
-  Global Instance Expr_ok : @ExprI.ExprOk typ RType_typ (expr typ func) Expr_expr := @ExprOk_expr _ _ _ _ _ _ _ _.
-
-  Require Import MirrorCore.VariablesI.
-  Require Import MirrorCore.Lambda.ExprVariables.
-
-  Global Instance ExprVar_expr : ExprVar (expr typ func) := _.
-  Global Instance ExprVarOk_expr : ExprVarOk ExprVar_expr := _.
-
-  Global Instance ExprUVar_expr : ExprUVar (expr typ func) := _.
-  Global Instance ExprUVarOk_expr : ExprUVarOk ExprUVar_expr := _.
-
-  Definition subst : Type :=
-    FMapSubst.SUBST.raw (expr typ func).
-  Global Instance SS : SubstI.Subst subst (expr typ func) :=
-    @FMapSubst.SUBST.Subst_subst _.
-  Global Instance SU : SubstI.SubstUpdate subst (expr typ func) :=
-    @FMapSubst.SUBST.SubstUpdate_subst _ _ _ _.
-Check SubstI.SubstOk.
-  Global Instance SO : @SubstI.SubstOk _ _ _ _ _ SS :=
-    @FMapSubst.SUBST.SubstOk_subst typ RType_typ (expr typ func) _.
-  Global Instance SUO : @SubstI.SubstUpdateOk _ _ _ _ _ _ SU SO :=  @FMapSubst.SUBST.SubstUpdateOk_subst typ RType_typ (expr typ func) _ _.
-
-End SimpleFunc.
-
-Section ReifyFunc.
-
-  Global Instance Reify_func : Reify (expr typ func) :=
-    Reify_func typ func (reify_nat typ func :: reify_list typ func :: reify_listOp typ func :: nil).
-
-End ReifyFunc.
-
-Definition rt := reify_scheme typ.
-Definition re := reify_scheme (expr typ func).
-
-Reify Declare Syntax patterns_simple_typ := rt.
-Reify Declare Syntax patterns_simple_expr := re.
-
-
-
-Ltac reify trm :=
-  let t := fresh "t" in
-  let k e := pose e as t
-  in
-  reify_expr patterns_simple_expr k [[ True ]] [[ trm ]]; cbv beta iota in t.
-
-Goal True.
-  reify (In 5 (5::4::3::nil)).
-
-  apply I.
-Qed.
-(*
-SearchAbout In.
-Require Import MirrorCore.Lemma.
-Require Import MirrorCore.Polymorphic.
-
-Instance Reify_lemma : Reify (lemma typ (expr typ func) (expr typ func)).
-Check @Reify_rlemma typ (expr typ func).
-Admitted.
-
-Definition lem_in_eq : polymorphic typ 1 (Lemma.lemma typ (expr typ func) (expr typ func)) :=
-Eval unfold Lemma.add_var, Lemma.add_prem, Lemma.vars, Lemma.concl, Lemma.premises in
-  <:: @in_eq ::>.
-
-SearchAbout Reify Lemma.lemma.
-
-
-
-
-unfold Lemma.mkLemma.
- :=
-  Eval unfold Lemma.add_var, Lemma.add_prem , Lemma.vars , Lemma.concl , Lemma.premises in
-*)
